ExhaleRel.thy
@@ -2,25 +2,27 @@ theory ExhaleRel
   imports ExpRel ExprWfRel TotalViper.ViperBoogieTranslationInterface Simulation
 begin
 
+abbreviation convert_rel
+  where "convert_rel R \<omega>0_\<omega> \<equiv> R (fst \<omega>0_\<omega>) (snd \<omega>0_\<omega>)"
+
 definition exhale_rel :: 
     "('a full_total_state \<Rightarrow> 'a full_total_state \<Rightarrow> 'b nstate \<Rightarrow> bool)
      \<Rightarrow> 'a total_context
         \<Rightarrow> ('a full_total_state \<Rightarrow> bool)
            \<Rightarrow> bigblock list \<Rightarrow> 'b econtext_bpl_general \<Rightarrow> (pure_exp, pure_exp atomic_assert) assert \<Rightarrow> bigblock \<times> cont \<Rightarrow> bigblock \<times> cont \<Rightarrow> bool"
   where "exhale_rel R ctxt_vpr StateCons P ctxt assertion_vpr \<gamma> \<gamma>' \<equiv>
-         rel_general (\<lambda>\<omega>0_\<omega>. R (fst \<omega>0_\<omega>) (snd \<omega>0_\<omega>)) (\<lambda>\<omega>0_\<omega>. R (fst \<omega>0_\<omega>) (snd \<omega>0_\<omega>))
+         rel_general (convert_rel R) (convert_rel R)
            \<comment>\<open>The well-definedness state remains the same\<close>
-           (\<lambda> \<omega>0_\<omega> \<omega>0_\<omega>'. (fst \<omega>0_\<omega>) = (fst \<omega>0_\<omega>') \<and> red_exhale ctxt_vpr StateCons (fst \<omega>0_\<omega>) assertion_vpr (snd \<omega>0_\<omega>) (ExhaleNormal (snd \<omega>0_\<omega>')))
-           (\<lambda> \<omega>0_\<omega>. red_exhale ctxt_vpr StateCons (fst \<omega>0_\<omega>) assertion_vpr (snd \<omega>0_\<omega>) ExhaleFailure)
+           (\<lambda> \<omega>0_\<omega> \<omega>0_\<omega>'. (fst \<omega>0_\<omega>) = (fst \<omega>0_\<omega>') \<and> red_exhale ctxt_vpr StateCons (fst \<omega>0_\<omega>) assertion_vpr (snd \<omega>0_\<omega>) (RNormal (snd \<omega>0_\<omega>')))
+           (\<lambda> \<omega>0_\<omega>. red_exhale ctxt_vpr StateCons (fst \<omega>0_\<omega>) assertion_vpr (snd \<omega>0_\<omega>) RFailure)
            P ctxt \<gamma> \<gamma>'"
-
 
 lemma exhale_rel_intro:
   assumes "\<And> \<omega>0 \<omega> \<omega>' ns. R \<omega>0 \<omega> ns \<Longrightarrow>
-                      red_exhale ctxt_vpr StateCons \<omega>0 assertion_vpr \<omega> (ExhaleNormal \<omega>') \<Longrightarrow>
+                      red_exhale ctxt_vpr StateCons \<omega>0 assertion_vpr \<omega> (RNormal \<omega>') \<Longrightarrow>
                       \<exists>ns'. red_ast_bpl P ctxt (\<gamma>, Normal ns) (\<gamma>', Normal ns') \<and> R \<omega>0 \<omega>' ns'" and
           "\<And> \<omega>0 \<omega> ns. R \<omega>0 \<omega> ns \<Longrightarrow>
-                      red_exhale ctxt_vpr StateCons \<omega>0 assertion_vpr \<omega> ExhaleFailure \<Longrightarrow>
+                      red_exhale ctxt_vpr StateCons \<omega>0 assertion_vpr \<omega> RFailure \<Longrightarrow>
                       \<exists>\<gamma>'. red_ast_bpl P ctxt (\<gamma>, Normal ns) (\<gamma>', Failure)"
   shows "exhale_rel R ctxt_vpr StateCons P ctxt assertion_vpr \<gamma> \<gamma>'"
   using assms
@@ -40,7 +42,7 @@ lemma exhal_rel_normal_elim:
 lemma exhale_rel_failure_elim:
   assumes "exhale_rel R ctxt_vpr StateCons P ctxt assertion_vpr \<gamma> \<gamma>'" and
           "R \<omega>0 m ns" and
-          "red_exhale ctxt_vpr StateCons \<omega>0 assertion_vpr m ExhaleFailure"
+          "red_exhale ctxt_vpr StateCons \<omega>0 assertion_vpr m RFailure"
         shows "\<exists>\<gamma>'. red_ast_bpl P ctxt (\<gamma>, Normal ns) (\<gamma>', Failure)"  
   using assms
   unfolding exhale_rel_def rel_general_def
@@ -96,9 +98,9 @@ proof (rule rel_general_cond[OF rev_iffD1_def[OF wf_rel_inst_eq_1[OF ExpWfRel] w
     apply fastforce
     by simp
 next
-  let ?Success = "\<lambda>\<omega> \<omega>'. fst \<omega> = fst \<omega>' \<and> red_exhale ctxt_vpr StateCons (fst \<omega>) (assert.Imp cond A) (snd \<omega>) (ExhaleNormal (snd \<omega>'))"
+  let ?Success = "\<lambda>\<omega> \<omega>'. fst \<omega> = fst \<omega>' \<and> red_exhale ctxt_vpr StateCons (fst \<omega>) (assert.Imp cond A) (snd \<omega>) (RNormal (snd \<omega>'))"
   let ?SuccessExp = "\<lambda>\<omega> \<omega>'. \<omega> = \<omega>' \<and> (\<exists>v. ctxt_vpr, StateCons, Some (fst \<omega>) \<turnstile> \<langle>cond;snd \<omega>\<rangle> [\<Down>]\<^sub>t Val v)"
-  let ?SuccessThn = "\<lambda>\<omega> \<omega>'. fst \<omega> = fst \<omega>' \<and> red_exhale ctxt_vpr StateCons (fst \<omega>) A (snd \<omega>) (ExhaleNormal (snd \<omega>'))"
+  let ?SuccessThn = "\<lambda>\<omega> \<omega>'. fst \<omega> = fst \<omega>' \<and> red_exhale ctxt_vpr StateCons (fst \<omega>) A (snd \<omega>) (RNormal (snd \<omega>'))"
   
   show "\<And> \<omega> \<omega>' ns. ?Success \<omega> \<omega>' \<Longrightarrow> R (fst \<omega>) (snd \<omega>) ns \<Longrightarrow>
                         ?SuccessExp \<omega> \<omega> \<and> \<comment>\<open>implicit assumption that success of conditional does not lead to side effects\<close>
@@ -120,8 +122,8 @@ next
       by (metis R prod_eqI val_rel_vpr_bpl.simps(2))
   qed
 
-  let ?Fail ="\<lambda>\<omega>. red_exhale ctxt_vpr StateCons (fst \<omega>) (assert.Imp cond A) (snd \<omega>) ExhaleFailure"
-  let ?FailThn = "\<lambda>\<omega>. red_exhale ctxt_vpr StateCons (fst \<omega>) A (snd \<omega>) ExhaleFailure"
+  let ?Fail ="\<lambda>\<omega>. red_exhale ctxt_vpr StateCons (fst \<omega>) (assert.Imp cond A) (snd \<omega>) RFailure"
+  let ?FailThn = "\<lambda>\<omega>. red_exhale ctxt_vpr StateCons (fst \<omega>) A (snd \<omega>) RFailure"
   let ?FailExp = "\<lambda>\<omega>. ctxt_vpr, StateCons, Some (fst \<omega>) \<turnstile> \<langle>cond;snd \<omega>\<rangle> [\<Down>]\<^sub>t VFailure"
 
  show "\<And> \<omega> ns. ?Fail \<omega> \<Longrightarrow> R (fst \<omega>) (snd \<omega>) ns \<Longrightarrow> 
